src/program_logic/staged_invariant.v
@@ -1,7 +1,7 @@
 From iris.algebra Require Import gmap auth agree gset coPset excl csum.
 From iris.base_logic.lib Require Export fancy_updates.
 From stdpp Require Export namespaces.
-From iris.base_logic.lib Require Import wsat invariants saved_prop.
+From iris.base_logic.lib Require Import wsat invariants ae_invariants saved_prop.
 From iris.algebra Require Import gmap.
 From iris.proofmode Require Import tactics.
 From Perennial.program_logic Require Export step_fupd_extra crash_token crash_weakestpre ae_invariants_mutable ghost_var.
@@ -42,24 +42,29 @@ Definition bi_sch_staged_cases :=
 Definition bi_sch_staged E :=
   bi_sch_sep (bi_sch_staged_fupd E) (bi_sch_staged_cases).
 
+Lemma bi_sch_staged_interp `{!invG Σ, !crashG Σ, !stagedG Σ} E k Qs P γ :
+  bi_schema_interp (S k) (bi_later <$> [C; P; staged_pending 1%Qp γ])
+                   (bi_later <$> [Qs]) (bi_sch_staged E)
+  ⊣⊢ ((▷ Qs ∧ (▷ C -∗ staged_pending 1%Qp γ -∗ |k,Some O={E}=> |k, Some O={∅, ∅}=> ▷ P)))%I.
+Proof. Admitted.
+
+(*
 Lemma bi_sch_staged_interp `{!invG Σ, !crashG Σ, !stagedG Σ} E k Qs Qr P :
   bi_schema_interp (S k) (bi_later <$> [C; P]) (bi_later <$> [Qs; Qr]) (bi_sch_staged E)
-  ⊣⊢ (((▷ Qs -∗ ▷ C -∗ |k={E}=> |k={∅, ∅}=> ▷ P ∗ ▷ Qr) ∗ ▷ Qs) ∨ (▷ Qr ∗ ▷ C ∗ ▷ P))%I.
+  ⊣⊢ ((▷ Qs ∧ (▷ C -∗ |k,Some O={E}=> |k, Some O={∅, ∅}=> ▷ P ∗ ▷ Qr)) ∨ (▷ Qr ∗ ▷ C ∗ ▷ P))%I.
 Proof. Admitted.
-(*
   remember (S k) as k' eqn:Hlvl.
   repeat (rewrite ?bi_schema_interp_unfold //=).
   rewrite /cfupd ?uPred_fupd_level_eq /uPred_fupd_level_def.
   rewrite Hlvl /bi_except_0 intuitionistically_into_persistently.
   done.
 Qed.
-*)
+ *)
 
-Lemma bi_sch_staged_interp_weak `{!invG Σ, !crashG Σ, !stagedG Σ} E k Qs_mut P :
-  bi_schema_interp (S k) (bi_later <$> [C; P]) (bi_later <$> Qs_mut) (bi_sch_staged E)
-  ⊣⊢ let Qs := default emp%I (bi_later <$> (Qs_mut !! O)) in
-     let Qr := default emp%I (bi_later <$> (Qs_mut !! 1)) in
-     ((((Qs -∗ ▷ C -∗ |k={E}=> |k={∅, ∅}=> ▷ P ∗ Qr) ∗ Qs) ∨ (Qr ∗ ▷ C ∗ ▷ P)))%I.
+Lemma bi_sch_staged_interp_weak `{!invG Σ, !crashG Σ, !stagedG Σ} E k Qs_mut P γ :
+  bi_schema_interp (S k) (bi_later <$> [C; P; staged_pending 1%Qp γ]) (bi_later <$> Qs_mut) (bi_sch_staged E)
+                   ⊣⊢ let Qs := default emp%I (bi_later <$> (Qs_mut !! O)) in
+                      (((Qs ∧  (▷ C -∗ staged_pending 1%Qp γ -∗ |k,Some O={E}=> |k, Some O={∅, ∅}=> ▷ P))))%I.
 Proof. Admitted.
 (*
   remember (S k) as k' eqn:Hlvl.
@@ -76,11 +81,20 @@ Section staged_inv_defns.
   Context `{!invG Σ, !crashG Σ, !stagedG Σ}.
 
 Definition staged_inv (k: nat) E (γ: gname) (P: iProp Σ) : iProp Σ :=
-  ae_inv_mut k (bi_sch_staged E) [C; (P ∨ staged_done γ)%I].
+  ae_inv_mut k None (bi_sch_staged E) [C; P; staged_pending 1%Qp γ].
 
-Definition staged_value (k: nat) E (γp: gname) (b: bool) (Qs Qr P: iProp Σ) :=
-  (∃ γr, (if b then staged_pending 1%Qp γr else staged_done γr) ∗
-  ae_inv_mut_full k (bi_sch_staged E) [Qs; (Qr ∨ staged_done γr)] [C; (P ∨ staged_done γp)%I])%I.
+Definition staged_value (k: nat) k2 mj2  E (γp: gname) (Qs Qr P: iProp Σ) :=
+  (∃ γcancel γr,
+  staged_pending 1%Qp γr ∗
+  staged_pending (1/2)%Qp γcancel ∗
+  ae_inv k2 (Some mj2) ((Qs ∨ ((Qr ∨ staged_done γr) ∗ C ∗ (P ∨ staged_done γp))) ∨ staged_done γcancel) ∗
+  ae_inv_mut_full k None (bi_sch_staged E) [staged_pending (1/2)%Qp γcancel] [C; P; staged_pending 1%Qp γp])%I.
+
+Definition staged_value_disc (k: nat) (mj: nat) (γp: gname) (Qs Qr P: iProp Σ) :=
+  (∃ γcancel γr,
+  staged_pending 1%Qp γr ∗
+  staged_pending (1/2)%Qp γcancel ∗
+  ae_inv k (Some mj) ((Qs ∨ ((Qr ∨ staged_done γr) ∗ C ∗ (P ∨ staged_done γp))) ∨ staged_done γcancel))%I.
 
 End staged_inv_defns.
 
@@ -142,105 +156,186 @@ Proof. by rewrite /staged_pending -own_op -Cinl_op frac_op' Qp_div_2. Qed.
 
 Lemma staged_inv_alloc k E E' P Q Qr:
   ▷ Q ∗ (C -∗ ▷ Q -∗ ▷ P ∗ ▷ Qr) -∗ |(S k)={E}=>
-  ∃ γ, staged_inv (S k) E' γ P ∗ staged_value (S k) E' γ true Q Qr P ∗ staged_pending 1%Qp γ.
+  ∃ γ, staged_inv (S k) E' γ P ∗ staged_value (S k) O O E' γ Q Qr P ∗ staged_pending 1%Qp γ.
 Proof.
-  iMod (pending_alloc) as (γ) "H".
+  iMod (pending_alloc) as (γp) "Hp".
+  iMod (pending_alloc) as (γcancel) "Hc".
   iMod (pending_alloc) as (γr) "Hr".
   iIntros "(HQ&HQP)".
-  iMod (ae_inv_mut_alloc (S k) E (bi_sch_staged E')
-                   [C; (P ∨ staged_done γ)%I]
-                   [Q; (Qr ∨ staged_done γr)%I]
-          with "[HQ HQP]")
-      as "(#Hi&Hmut)".
+  rewrite uPred_fupd_level_eq.
+  iPoseProof (ae_inv_alloc' O (Some O) E
+        (((Q ∨ ((Qr ∨ staged_done γr) ∗ C ∗ (P ∨ staged_done γp))) ∨ staged_done γcancel))%I
+        with "[HQ]") as "H".
+  { repeat iLeft. auto. }
+  iDestruct (pending_split with "Hc") as "(Hc1&Hc2)".
+  iMod (fupd_split_level_le with "H") as "#Hinv0".
+  { lia. }
+
+  iMod (ae_inv_mut_alloc (S k) None E (bi_sch_staged E')
+                         [C; P; staged_pending 1%Qp γp]
+                         [staged_pending (1/2)%Qp γcancel]
+          with "[Hc1 HQP]")
+    as "(#Hi&Hmut)".
   { simpl fmap. rewrite bi_sch_staged_interp.
-    iLeft.
-    iSplitL "HQP".
-    - iIntros "HQ >HC". iModIntro.
-      iApply fupd_level_mask_weaken; first by set_solver+.
-      iDestruct ("HQP" with "[$] [$]") as "($&$)".
-    - eauto.
+    iSplit; first iFrame.
+    iIntros ">#HC Hpend".
+    iPoseProof (ae_inv_acc E' _ _ _ (▷ P) with "Hinv0 [Hc1 HQP Hpend]") as "H".
+    { iIntros "[HQ|>Hfalse]"; last first.
+      { iDestruct (pending_done with "Hc1 [$]") as %[]. }
+      iDestruct "HQ" as "[HQ|H]".
+      { iDestruct ("HQP" with "[$] [$]") as "($&HQr)".
+        iMod (pending_upd_done with "Hpend") as "#Hdone".
+        iModIntro. iLeft. iRight. iFrame "# ∗".
+      }
+      iDestruct "H" as "(HQ&_&[HP|>Hfalse])"; last first.
+      { iDestruct (pending_done with "Hpend [$]") as %[]. }
+      iMod (pending_upd_done with "Hpend") as "#Hdone".
+      iModIntro. iFrame "HP". iLeft. iFrame "# ∗".
+    }
+    iMod (fupd_split_level_le with "H"); first (naive_solver lia).
+    iFrame. eauto.
   }
-  iModIntro. iExists _. iFrame "# ∗". iExists _; eauto. iFrame.
+  iModIntro. iExists _. iFrame "# ∗". iExists _, _. iFrame "# ∗".
 Qed.
 
-(* TODO: need t o be able to get something back if we don't fire the view shift. And what about the Qr case? *)
-Lemma staged_inv_open_modify_ae E k E1 γ P Q Qr Q' Qr' R:
-  staged_value (S k) E1 γ true Q Qr P -∗
-  (▷ Q -∗ |k={E}=> (▷ Q' -∗ |C={E1, ∅}_k=> P ∗ Qr') ∗  ▷ Q' ∗ R) -∗
-  |(S k)={E}=> (R ∗ staged_value (S k) E1 γ true Q' Qr' P) ∨
-               (▷ Qr ∗ C ∗ staged_value (S k) E1 γ false Q' Qr' P).
+Lemma staged_inv_open_modify_ae E k k2 k2' j j' E1 γ P Q Qr Q' Qr' R:
+  k2 ≤ k →
+  k2' ≤ k →
+  staged_value (S k) k2 j E1 γ Q Qr P -∗
+  (▷ Q -∗ |k,Some O={E}=> (▷ Q' -∗ C -∗ |k2',Some (S j')={E1}=> |k2',Some (S j')={∅, ∅}=> P ∗ Qr') ∗  ▷ Q' ∗ R) -∗
+  |(S k)={E}=> (R ∗ staged_value (S k) k2' j' E1 γ Q' Qr' P) ∨
+               (▷ Qr ∗ C).
 Proof.
-  iIntros "Hval Hshift".
+  iIntros (Hle Hle') "Hval Hshift".
   rewrite /staged_value/=.
-  iDestruct "Hval" as (γr) "(Hγr&Hval)" => //=.
-  iMod (ae_inv_mut_full_acc _ _ _ _ ([Q'; (Qr' ∨ staged_done γr)%I]) _
-                            ((R ∗ staged_pending 1%Qp γr)  ∨ (▷ Qr ∗ C ∗ staged_done γr))%I
-          with "Hval [Hγr Hshift]") as "(HR&Hclo)";
+  iMod (pending_alloc) as (γcancel') "Hc".
+  iDestruct (pending_split with "Hc") as "(Hc1&Hc2)".
+  iDestruct "Hval" as (γcancel γr) "(Hγr&Hcancel&#Hinv0&Hval)" => //=.
+  iEval (rewrite uPred_fupd_level_eq).
+  iMod (ae_inv_mut_full_acc _ _ _ _ _ ([staged_pending (1/2)%Qp γcancel']) _
+                            (((R ∗ staged_pending 1%Qp γr ∗
+                                 ae_inv k2' (Some j') ((Q' ∨ (Qr' ∨ staged_done γr) ∗ C ∗ (P ∨ staged_done γ))
+                                                         ∨ staged_done γcancel')))
+                             ∨
+                            (((▷ Qr ∗ staged_done γr ∗ C))))%I
+          with "Hval [Hcancel Hγr Hshift Hc1]") as "(HR&Hclo)";
     last first.
-  { iModIntro. iDestruct "Hclo" as "[(Hr&?)|(?&?&?)]".
-    - iLeft. iFrame. iExists _. iFrame; eauto.
-    - iRight. iFrame. iExists _. iFrame; eauto.
+  { iModIntro. iDestruct "Hclo" as "[(Hr&?&#Hinv)|(?&?&?)]".
+    - iLeft. iFrame. iExists _, _. iFrame; eauto.
+    - iRight. iFrame.
   }
   iIntros "HQ".
   iDestruct (bi_sch_staged_interp with "HQ") as "HQ".
-  iDestruct "HQ" as "[(Hwand&HQ)|HQ]".
-  - iMod ("Hshift" with "HQ") as "(Hwand2&HQ&HR)".
-    iSplitL "HQ Hwand2".
-    { iModIntro. erewrite bi_sch_staged_interp.
-      iLeft. iFrame "HQ".
-      iIntros "HQ' >HC". iMod ("Hwand2" with "[$] [$]") as "H".
-      iModIntro. by iMod "H" as "($&$)".
-    }
-    iModIntro. iLeft. iFrame.
-  - iDestruct "HQ" as "(HQr&>#HC&HP)".
-    iDestruct "HQr" as "[HQR|>Hfalse]"; last first.
-    { iDestruct (pending_done with "[$] [$]") as %[]. }
-    iMod (pending_upd_done with "Hγr") as "#Hγr".
+  iDestruct "HQ" as "(>Hcancel'&_)".
+
+  (* Cancel the old invariant *)
+  iDestruct (pending_join with "[$Hcancel $Hcancel']") as "Hcancel".
+  iPoseProof (ae_inv_acc E _ _ _ (▷ (Q ∨ (Qr ∨ staged_done γr) ∗ C ∗ (P ∨ staged_done γ)))
+                with "Hinv0 [Hcancel]") as "H".
+  { iIntros "[Hleft|>Hfalse]".
+    { iMod (pending_upd_done with "Hcancel"). iModIntro. iSplitR "Hleft"; last by iFrame.
+      iFrame "∗". }
+    iDestruct (pending_done with "[$] [$]") as %[].
+  }
+  iClear "Hinv0".
+  iMod (fupd_split_level_le with "H") as "H".
+  { naive_solver lia. }
+  iDestruct "H" as "[HQ|HQ]".
+  - iMod ("Hshift" with "[$]") as "(Hwand&HQ'&HR)".
+    iPoseProof (ae_inv_alloc' k2' (Some j') E
+        (((Q' ∨ ((Qr' ∨ staged_done γr) ∗ C ∗ (P ∨ staged_done γ))) ∨ staged_done γcancel'))%I
+        with "[HQ']") as "H".
+    { repeat iLeft. auto. }
+    iMod (fupd_split_level_le with "H") as "#Hinv".
+    { naive_solver lia. }
     iModIntro.
-    iSplitL "Hshift HP".
-    { rewrite bi_sch_staged_interp.
-      iRight. iFrame. eauto.
+    rewrite bi_sch_staged_interp. iFrame "Hinv".
+    iSplitR "HR Hγr"; last first.
+    { iLeft. by iFrame. }
+    iSplit; first iFrame.
+    iIntros ">#HC Hpend".
+
+    iPoseProof (ae_inv_acc E1 _ _ _ (▷ P) with "Hinv [Hc1 Hpend Hwand]") as "H".
+    { iIntros "HQ".
+      iDestruct "HQ" as "[HQ|>Hfalse]"; last first.
+      { iDestruct (pending_done with "Hc1 Hfalse") as %[]. }
+      iDestruct "HQ" as "[HQ|HQ]".
+      * iMod ("Hwand" with "[$] [$]") as "Hwand".
+        iMod (fupd_split_level_intro_mask' _ ∅) as "Hclo''"; first by set_solver+.
+        iMod ("Hwand") as "(HP&HQr')".
+        iMod (pending_upd_done with "Hpend").
+        iMod "Hclo''" as "_".
+        iModIntro. iFrame "HP". iNext. iFrame "HC". iLeft.
+        iRight. iFrame.
+      * iDestruct "HQ" as "(HQr&_&[HP|>Hfalse])"; last first.
+        { iDestruct (pending_done with "Hpend Hfalse") as %[]. }
+        iMod (pending_upd_done with "Hpend").
+        iModIntro. iFrame "HP". iNext. iFrame "HC". iLeft.
+        iRight. iFrame.
     }
-    iRight. iFrame "# ∗".
+    iMod (fupd_split_level_le with "H"); first (naive_solver lia).
+    do 2 iModIntro; eauto.
+  - iDestruct "HQ" as "([HQr|>Hfalse]&#>HC&HP)"; last first.
+    { iDestruct (pending_done with "Hγr Hfalse") as %[]. }
+    iMod (pending_upd_done with "Hγr") as "#Hγr".
+    iPoseProof (ae_inv_alloc' k2' (Some j') E
+        (((((Qr' ∨ staged_done γr) ∗ C ∗ (P ∨ staged_done γ))) ∨ staged_done γcancel'))%I
+        with "[Hγr HP]") as "H".
+    { iLeft. iFrame. eauto. }
+    iMod (fupd_split_level_le with "H") as "#Hinv".
+    { naive_solver lia. }
+    iModIntro.
+    rewrite bi_sch_staged_interp.
+    iSplitR "HQr Hγr"; last first.
+    { iRight. iFrame "# ∗". }
+    iSplit; first iFrame.
+    iIntros "_ Hpend".
+    iPoseProof (ae_inv_acc E1 _ _ _ (▷ P) with "Hinv [Hc1 Hpend]") as "H".
+    { iIntros "HQ".
+      iDestruct "HQ" as "[HQ|>Hfalse]"; last first.
+      { iDestruct (pending_done with "Hc1 Hfalse") as %[]. }
+      iDestruct "HQ" as "(HQr&_&[HP|>Hfalse])"; last first.
+      { iDestruct (pending_done with "Hpend Hfalse") as %[]. }
+      iMod (pending_upd_done with "Hpend").
+      iModIntro. iFrame "HP". iNext. iFrame "HC". iLeft.
+      iFrame.
+    }
+    iMod (fupd_split_level_le with "H"); first (naive_solver lia).
+    do 2 iModIntro; eauto.
 Qed.
 
-(* XXX: this is not currently true, but a better encoding of inv_mut should enable that *)
-Lemma staged_value_into_disc k E γ P Q Qr :
-  staged_value k E γ true Q Qr P -∗
-  <disc> staged_value k E γ true Q Qr P.
-Proof. Admitted.
-
-Lemma staged_inv_open_crash k E γ P Q Qr:
-  (▷ Q -∗ ▷ C -∗ |k={E}=> |k={∅, ∅}=> ▷ P ∗ ▷ Qr) -∗
-  staged_value (S k) E γ true Q Qr P -∗ C -∗ |(S k)={E,E}=> ▷ Qr.
+Lemma staged_value_into_disc k k2 mj2 E γ P Q Qr :
+  staged_value k k2 mj2 E γ Q Qr P -∗
+  <disc> staged_value_disc k2 mj2 γ Q Qr P.
 Proof.
-  iIntros "Hwand".
-  iDestruct 1 as (?) "(Hγr&Hval)". iIntros "#HC".
-  iMod (ae_inv_mut_full_acc _ _ _ _ ([Q; (Qr ∨ staged_done γr)%I]) _
-                            (▷ Qr)%I
-          with "Hval [Hγr]") as "(HR&Hclo)";
-    last first.
-  { iModIntro. auto. }
+  iDestruct 1 as (??) "(Hp1&Hp2&#Hinv&_)".
+  iModIntro. iExists _, _. by iFrame.
+Qed.
+
+Lemma staged_inv_disc_open_crash k mj E γ P Q Qr:
+  □ (▷ Q -∗ ▷ C -∗ |k, Some (S mj)={E}=> |k, Some (S mj)={∅, ∅}=> ▷ P ∗ ▷ Qr) -∗
+  staged_value_disc k mj γ Q Qr P -∗ C -∗ |k, Some mj={E}=> ▷ Qr.
+Proof.
+  iIntros "#Hwand".
+  iDestruct 1 as (??) "(Hqr&Hqc&#Hinv)".
+  iIntros "#HC".
+  iMod (ae_inv_acc _ _ _ _ (▷ Qr)%I
+          with "Hinv [Hqr Hqc]") as "$"; last done.
   iIntros "HQ".
-  iDestruct (bi_sch_staged_interp with "HQ") as "HQ".
-  iDestruct "HQ" as "[(Hwand'&HQ)|HQ]".
-  - iMod ("Hwand'" with "[$] [$]") as "H".
-    iMod (fupd_level_intro_mask' _ ∅) as "Hclo''"; first by set_solver+.
-    iMod ("H") as "(HP&Hdone)".
+  iDestruct "HQ" as "[HQ|>Hfalse]"; last first.
+  { iDestruct (pending_done with "[$] [$]") as %[]. }
+  iDestruct "HQ" as "[HQ|HQ]".
+  - iMod ("Hwand" with "[$] [$]") as "H".
+    iMod (fupd_split_level_intro_mask' _ ∅) as "Hclo''"; first by set_solver+.
+    iMod ("H") as "(HP&HQr)".
     iMod "Hclo''" as "_".
-    iDestruct "Hdone" as "[HQR|>Hfalse]"; last first.
-    { iDestruct (pending_done with "[$] [$]") as %[]. }
-    iMod (pending_upd_done with "Hγr") as "Hγr".
-    iModIntro. rewrite bi_sch_staged_interp. iFrame "#". iFrame.
+    iMod (pending_upd_done with "Hqr") as "#Hdone".
+    iModIntro. iFrame "HQr". iLeft. iRight. iFrame "# ∗".
   - iDestruct "HQ" as "([HQr|>Hfalse]&_&HP)"; last first.
-    { iDestruct (pending_done with "Hγr [$]") as %[]. }
-    iMod (pending_upd_done with "Hγr") as "#Hγr".
-    iModIntro.
-    iSplitL "HP".
-    { rewrite bi_sch_staged_interp.
-      iRight. iFrame "# ∗".
-    }
-    eauto.
+    { iDestruct (pending_done with "Hqr [$]") as %[]. }
+    iMod (pending_upd_done with "Hqr") as "#Hdone".
+    iModIntro. iFrame "HQr".
+    iLeft. iRight. iFrame "# ∗".
 Qed.
 
 Lemma staged_inv_weak_open E k E1 γ P:
@@ -250,10 +345,12 @@ Lemma staged_inv_weak_open E k E1 γ P:
   C -∗ |(S k)={E,E}=> ▷ P.
 Proof.
   iIntros (?) "(#Hinv&Hpending&#HC)".
-  iMod (ae_inv_mut_acc _ _ _ _ (▷ P) with "Hinv [Hpending]"); last done.
+  rewrite /staged_inv.
+  rewrite uPred_fupd_level_eq.
+  iMod (ae_inv_mut_acc _ _ _ _ _ (▷ P) with "Hinv [Hpending]"); last done.
   iIntros (Qs) "Hinv0".
   iDestruct (bi_sch_staged_interp_weak with "Hinv0") as "H".
-  iDestruct "H" as "[(Hwand&HQ)|HQ]".
+  iDestruct "H" as "(_&Hwand)".
   - iMod (fupd_level_intro_mask' _ E1) as "Hclo''"; auto.
     iDestruct ("Hwand" with "[$] [$]") as "Hwand".
     iMod (fupd_level_le with "Hwand") as "Hwand"; auto.
