src/program_logic/crash_adequacy.v
@@ -31,10 +31,14 @@ Proof.
   rewrite {1}wpc_unfold /wpc_pre. iIntros (?) "Hσ H HNC".
   rewrite (val_stuck e1 σ1 κ e2 σ2 efs) //.
   iSpecialize ("H" $! O).
+  Search _ bi_forall bi_sep.
   iMod "H". iDestruct "H" as "(H&_)".
   iMod ("H" $! _ σ1 with "Hσ HNC") as "(_&H)".
   iMod ("H" $! e2 σ2 efs with "[//]") as "H".
-  by do 2 iModIntro.
+  do 2 iModIntro. iMod "H" as "($&Hwpc&?&$)". iModIntro.
+  iSplitL "Hwpc".
+  - rewrite wpc_eq. iIntros (mj). iApply (wpc0_strong_mono with "Hwpc"); auto.
+    { }naive_solver lia. 
 Qed.
 
 Lemma wptp_step s k e1 t1 t2 κ κs σ1 σ2 Φ Φc :
